Test.dfy
@@ -1,6 +1,31 @@
 include "Rope.dfy"
 import opened Rope
 
+method quickstart()
+{
+    // initializing
+    var n1: Rope := new Rope.Terminal("Hello ");
+    var n2: Rope := new Rope.Terminal("world!");
+    // concat
+    var n: Rope := Rope.concat(n1, n2);
+    assert n.Valid();
+    // toString
+    var nstr: string := n.toString();
+    assert nstr == "Hello world!";
+    // length
+    assert n.length() == |nstr|;
+    // getCharAtIndex
+    var c: char := n.getCharAtIndex(n.length() - 1);
+    assert c == '!';
+    // report: returns a string
+    var fstr: string := n.report(0, 5);
+    assert fstr == "Hello";
+    // substring: returns a Rope
+    var first: Rope := Rope.substring(n, 0, 5);
+    var firstStr: string := first.toString();
+    assert firstStr == "Hello";
+}
+
 method test()
 {
     var n := new Rope.Terminal("Hello ");
